Actual proofs (random stashing)
Originally https://github.com/dfinity-lab/ic-ref/commit/d47fcfa7ca059f74c9b33184cc524042be6476cb

proofs/theories/IC/Ref.v
@@ -1,5 +1,225 @@
+Require Import Control.Monad.Trans.State.Lazy.
+Require Import Data.Functor.Identity.
+
 Require Import IC.Ref.
+Require Import IC.Types.
+Require Import Data.Map.Internal.
 
 Import GHC.Base.
+Import GHC.Base.Notations.
+Import List.Notations.
 
 Set Bullet Behavior "Strict Subproofs".
+
+Ltac expand_pairs :=
+  match goal with
+    |- context[let (_,_) := ?e in _] =>
+    rewrite (surjective_pairing e)
+  end.
+
+Ltac destruct_match :=
+  match goal with
+  | [ H :context[match ?a with _ => _ end] |- _] =>
+    let Heq := fresh "Heq" in
+    destruct a eqn:Heq
+  | [ |- context[match ?a with _ => _ end]] =>
+    let Heq := fresh "Heq" in
+    destruct a eqn:Heq
+  end.
+
+(* Lemmas about State *)
+
+Lemma runState_state:
+  forall A B (f : A -> (B * A)) s, runState (state f) s = f s.
+Proof. intros. reflexivity. Qed.
+
+Lemma runState_return:
+  forall S A (x : A) (s : S), runState (return_ x) s = (x,s).
+Proof. intros. reflexivity. Qed.
+
+Lemma runState_bind:
+  forall S A B (m1 : State S A) (m2 : A -> State S B) (s : S),
+  runState (m1 >>= m2) s = 
+    let (x, s') := runState m1 s in
+    runState (m2 x) s'.
+Proof. intros.
+  destruct m1 as [m1].
+  repeat unfold runState, Base.op_z2218U__, runIdentity, runStateT,
+    op_zgzgze__, Monad__StateT, op_zgzgze____, Lazy.Monad__StateT_op_zgzgze__,
+    op_zgzgze__, Monad__Identity, op_zgzgze____, Identity.Monad__Identity_op_zgzgze__.
+  destruct (m1 s) as [ms].
+  destruct ms.
+  reflexivity.
+Qed.
+
+Lemma runState_then:
+  forall S A B (m1 : State S A) (m2 : State S B) (s : S),
+  runState (m1 >> m2) s = 
+    let s' := snd (runState m1 s) in
+    runState m2 s'.
+Proof. intros.
+  destruct m1 as [m1].
+  repeat unfold runState, Base.op_z2218U__, runIdentity, runStateT,
+    op_zgzg__, Monad__StateT, op_zgzg____, Lazy.Monad__StateT_op_zgzg__,
+    Lazy.Monad__StateT_op_zgzgze__,
+    op_zgzg__, Monad__Identity, op_zgzg____, Identity.Monad__Identity_op_zgzg__.
+  destruct (m1 s) as [ms].
+  destruct ms.
+  reflexivity.
+Qed.
+
+
+Lemma runState_gets:
+  forall A B C (f : A -> B) (m : B -> StateT _ Identity C) (s : A),
+  runState (gets f >>= m) s = runState (m (f s)) s.
+Proof. intros. reflexivity. Qed.
+
+
+Lemma onReject_liftRM_then:
+  forall A B f (g : M A) (h : RM B) s,
+  runState (onReject f (liftRM g >> h)) s = runState (g >> onReject f h) s.
+Proof.
+  intros.
+  destruct g as [g].
+  repeat unfold onReject, Except.runExceptT, liftRM, Class.lift,
+    op_zgzgze__, op_zgzg__, Monad__StateT,
+    Lazy.Monad__StateT_op_zgzgze__, op_zgzgze____, op_zgzg____,
+    Lazy.Monad__StateT_op_zgzg__, Lazy.Monad__StateT_op_zgzgze__,
+    runState, Base.op_z2218U__, runIdentity, runStateT,
+    Except.Monad__ExceptT,  Except.Monad__ExceptT_op_zgzg__,
+    Except.Monad__ExceptT_op_zgzgze__, Except.MonadTrans__ExceptT,
+    Except.runExceptT, Except.MonadTrans__ExceptT_lift,
+    Class.lift__, Monad__Identity, Identity.Monad__Identity_op_zgzgze__,
+    liftM, return_, return___, Lazy.Monad__StateT_return_, pure, 
+    Applicative__StateT, pure__, Lazy.Applicative__StateT_pure,
+    Identity.Monad__Identity_return_, Applicative__Identity,
+    Identity.Applicative__Identity_pure.
+  destruct (g s) as [gs].
+  destruct gs.
+  reflexivity.
+Qed.
+
+Lemma onReject_liftRM_bind:
+  forall A B f (g : M A) (h : A -> RM B) s,
+  runState (onReject f (liftRM g >>= h)) s = runState (g >>= (fun x => onReject f (h x))) s.
+Proof.
+  intros.
+  destruct g as [g].
+  repeat unfold onReject, Except.runExceptT, liftRM, Class.lift,
+    op_zgzgze__, op_zgzg__, Monad__StateT,
+    Lazy.Monad__StateT_op_zgzgze__, op_zgzgze____, op_zgzg____,
+    Lazy.Monad__StateT_op_zgzg__, Lazy.Monad__StateT_op_zgzgze__,
+    runState, Base.op_z2218U__, runIdentity, runStateT,
+    Except.Monad__ExceptT,  Except.Monad__ExceptT_op_zgzg__,
+    Except.Monad__ExceptT_op_zgzgze__, Except.MonadTrans__ExceptT,
+    Except.runExceptT, Except.MonadTrans__ExceptT_lift,
+    Class.lift__, Monad__Identity, Identity.Monad__Identity_op_zgzgze__,
+    liftM, return_, return___, Lazy.Monad__StateT_return_, pure, 
+    Applicative__StateT, pure__, Lazy.Applicative__StateT_pure,
+    Identity.Monad__Identity_return_, Applicative__Identity,
+    Identity.Applicative__Identity_pure.
+  destruct (g s) as [gs].
+  destruct gs.
+  reflexivity.
+Qed.
+
+Lemma runState_onReject_return:
+  forall A f (x : A) s,
+  runState (onReject f (return_ x)) s = (x,s).
+Proof. intros. reflexivity. Qed.
+
+
+Lemma runState_onReject_throwE:
+  forall A B f x (h : RM A) s,
+  runState (onReject f ((Except.throwE x : RM B) >> h)) s = runState (f x) s.
+Proof. intros. reflexivity. Qed.
+
+Lemma pure_then_RM:
+  forall A B f (x : A) (a : RM B) s,
+  runState (onReject f (pure x >> a)) s = runState (onReject f a) s.
+Proof. intros. reflexivity. Qed.
+
+Lemma reassoc_bind_bind_RM:
+  forall A B C f s (a : RM A) (b : A -> RM B) (c : B -> RM C),
+  runState (onReject f ((a >>= b) >>= c)) s
+  = runState (onReject f (a >>= b >>= c)) s.
+Admitted.
+
+
+Definition ICInvariant Q P :=
+  P initialIC /\
+  (forall rid pk r s0, 
+    P s0 ->
+    Q pk r ->
+    evalState (authAsyncRequest pk r) s0 = true ->
+    P (execState (submitRequest rid r) s0)) /\
+  (forall s0,
+    P s0 ->
+    P (execState runStep s0)).
+
+
+Definition any_request (pk : Blob) (r : AsyncRequest) := True.
+
+Theorem no_empty_canister_id :
+  ICInvariant any_request (fun s =>
+    member (Mk_EntityId nil) (canisters s) = false).
+Proof.
+  split; [|split].
+  * reflexivity.
+  * intros.
+    unfold submitRequest.
+    unfold execState.
+    unfold modify.
+    rewrite runState_state.
+    unfold snd.
+    destruct_match.
+    + assumption.
+    + destruct s0. assumption.
+  * intros.
+    unfold runStep.
+    unfold nextReceived.
+    unfold execState.
+    rewrite runState_gets.
+    destruct_match.
+    + destruct p as [rid ar].
+      rewrite runState_then.
+      rewrite runState_return.
+      simpl.
+      unfold processRequest.
+      destruct_match.
+      - unfold op_zezlzl__.
+        destruct_match.
+        ** rewrite runState_bind.
+           rewrite onReject_liftRM_bind.
+           rewrite runState_gets.
+           rewrite onReject_liftRM_bind.
+           rewrite runState_gets.
+           match goal with | [ |- context[when ?P] ] => destruct P eqn:Hwhen end.
+           ++ unfold when.
+              unfold reject.
+              rewrite runState_onReject_throwE.
+              simpl.
+              destruct s0. simpl. assumption.
+           ++ unfold when. rewrite pure_then_RM.
+              rewrite onReject_liftRM_then.
+              unfold createEmptyCanister.
+              rewrite runState_then.
+              unfold modify. rewrite runState_state.
+              unfold snd.
+              rewrite runState_onReject_return.
+              unfold setReqStatus.
+              unfold modify. rewrite runState_state.
+              unfold Base.op_z2218U__ in *.
+              destruct s0.
+              simpl.
+              (* now need theory about member and insert *)
+              (* and that freshid is not nil *)
+              admit.
+        ** admit. (* Cannot prove this, need to rule out ForcedChoice *)
+        ** rewrite runState_bind.
+           match goal with | [ |- context[Monad.unless ?P] ] => destruct P eqn:Hunless end.
+           ++ unfold Monad.unless.
+              (* need monad laws. Maybe see if with FunExt we can instantiate
+                 GHC.Base.MonadLaws *)
+Admitted.              
+              
